#+title: Solutions to Exercises 1.1 to 1.5 of Pedoe's "Geometry: A Comprehensive Course"
#+author: Joel McBride
#+options: num:nil toc:nil

* 1.1
Let \( P = (x_1, x_2) \), \( Q = (y_1, y_2) \), \( R = (z_1, z_2) \), \( S = (t_1, t_2) \).
By definition, \( \vec{PQ} = \vec{RS} \) iff \( (y_1-x_1, y_2-x_2) = (t_1-z_1, t_2-z_2) \).

** Reflexive property
   "\( \vec{PQ} = \vec{PQ} \)" means "\( y_1 - x_1 = y_1 - x_1 \) and \( y_2 - x_2 = y_2 - x_2 \)" which holds by reflexivity of algebraic equality.

** Symmetric property
   "If \( \vec{PQ} = \vec{RS} \) then \( \vec{RS} = \vec{PQ} \)" means algebraically "if \( y_1 - x_1 = t_1 - z_1 \) and \( y_2 - x_2 = t_2 - z_2 \) then \( t_1 - z_1 = y_1 - x_1 \) and \( t_2 - z_2 = y_2 - x_2 \)" which holds by symmetry of algebraic equality.

** Transitive property
   "If \( \vec{PQ} = \vec{RS} \) and \( \vec{RS} = \vec{TU} \) then \( \vec{PQ} = \vec{TU} \)" means algebraically
   
   if

   \begin{align}
   y_1 - x_1 = t_1 - z_1
   \end{align}

   and

   \begin{align}
   y_2 - x_2 = t_2 - z_2
   \end{align}

   and

   \begin{align}
   t_1 - z_1 = v_1 - u_1
   \end{align}

   and

   \begin{align}
   t_2 - z_2 = v_2 - u_2
   \end{align}

   then
   
   \begin{align}
   y_1 - x_1 = v_1 - u_1
   \end{align}  
   
   and

   \begin{align}
   y_2 - x_2 = v_2 - u_2
   \end{align}

   which holds by transitivity of Equation 1 and Equation 3 and of Equation 2 and Equation 4.

* 1.3
** \( P + (Q + R) = (P + Q) + R \)
   The parallelogram with sides \( P \) and \( Q + R \) has the same diagonal as the parallelogram with sides \( P + Q \) and \( R \).

** \( r(P + Q) = rP + rQ \)
   Stretching the diagonal of the parallelogram with sides \( P \) and \( Q \) by \( r \) is the same as stretching each side by \( r \).
   
* 1.4
\( (P + Q)/2 \) is the midpoint of the line segment \( PQ \).

* 1.5
Let \( U_1 = (a_1, a_2) \) and \( U_2 = (b_1, b_2) \).
We will show that numbers \( q_1 \) and \( q_2 \) can be found such that \( P = (x_1, x_2) = q_1U_1 + q_2U_2 \).

\( q_1U_1 + q_2U_2 = (q_1a_1 + q_2b_1, q_1a_2 + q_2b_2) \)

so we have the equations

\begin{align}
x_1 = q_1a_1 + q_2b_1
\end{align}

\begin{align}
x_2 = q_1a_2 + q_2b_2
\end{align}

Equation 7 x a_2 - Equation 8 x a_1 results in \( q_2 = \frac{a_2x_1 - a_1x_2}{b_1a_2 - b_2a_1} \).
Equation 7 x b_2 - Equation 8 x b_1 results in \( q_1 = \frac{b_2x_1 - b_1x_2}{a_1b_2 - a_2b_1} \).

Since \( U_1 \) and \( U_2 \) are independent \( b_1a_2 - b_2a_1 \) never equals 0 so numbers \( q_1 \) and \( q_2 \) can always be found.



   
   
