#+title: Solutions to Exercises 3.1 to 3.3 of Pedoe's "Geometry: A Comprehensive Course"
#+author: Joel McBride
#+options: num:nil toc:nil

* 3.1
#+attr_html: :width 150px
#+attr_latex: :width 150px
[[./fig-exercise-3.1.svg.png]]

* 3.2
Equivalent by \( k=1-t \) and \( k'=t \). 
If \( k + k' \neq 0 \) then we can divide and multiply by \( k + k' \) yielding \( \frac{k}{k+k'}((k+k')A) + \frac{k'}{k+k'}((k+k')B) \) which means \( C \) lies on the line defined by the points \( (k+k')A \) and \( (k+k')B \).

* 3.3
If \( E = \frac{A+C}{2} \) and \( D = \frac{B+C}{2} \) we will show \( E - D = k(A - B) \).

\begin{align*}
&E - D \\
&= \frac{A+C}{2} - \frac{B+C}{2} \\
&= \frac{1}{2} (A - B) 
\end{align*}

Therefore \( DE \) is parallel to \( BA \).
